mark-and-sweep/spec/GC.Spec.MajorHeap.Member.fst
@@ -1,0 +1,30 @@
+module GC.Spec.MajorHeap.Member
+
+module Seq = FStar.Seq
+module MH = GC.Spec.MajorHeap
+
+open GC.Spec.Base
+
+#push-options "--split_queries always --z3rlimit 5 --fuel 1 --ifuel 1"
+let major_objects_member_at_index_small
+  (mh: MH.major_heap) (idx: nat) (x: obj_addr)
+  : Lemma
+      (requires
+        idx < Seq.length mh /\
+        Seq.mem x (MH.objects_in_chunk (Seq.index mh idx)))
+      (ensures Seq.mem x (MH.major_objects mh))
+  =
+  MH.major_objects_member_at_index mh idx x
+
+let major_objects_member_at_equal_index_small
+  (mh: MH.major_heap) (idx: nat) (c: MH.heap_chunk) (x: obj_addr)
+  : Lemma
+      (requires
+        idx < Seq.length mh /\
+        Seq.index mh idx == c /\
+        Seq.mem x (MH.objects_in_chunk c))
+      (ensures Seq.mem x (MH.major_objects mh))
+  =
+  assert (Seq.mem x (MH.objects_in_chunk (Seq.index mh idx)));
+  major_objects_member_at_index_small mh idx x
+#pop-options
