mark-and-sweep/spec/GC.Spec.MajorHeap.Member.fsti
@@ -1,0 +1,28 @@
+module GC.Spec.MajorHeap.Member
+
+module Seq = FStar.Seq
+module MH = GC.Spec.MajorHeap
+
+open GC.Spec.Base
+
+val major_objects_member_at_index_small:
+  mh:MH.major_heap ->
+  idx:nat ->
+  x:obj_addr ->
+  Lemma
+    (requires
+      idx < Seq.length mh /\
+      Seq.mem x (MH.objects_in_chunk (Seq.index mh idx)))
+    (ensures Seq.mem x (MH.major_objects mh))
+
+val major_objects_member_at_equal_index_small:
+  mh:MH.major_heap ->
+  idx:nat ->
+  c:MH.heap_chunk ->
+  x:obj_addr ->
+  Lemma
+    (requires
+      idx < Seq.length mh /\
+      Seq.index mh idx == c /\
+      Seq.mem x (MH.objects_in_chunk c))
+    (ensures Seq.mem x (MH.major_objects mh))
